Append an IPC buffer translation and related lemma to the label mapping.
We need these later on when instantiating the CAmkES->CapDL generation locale,
and it is simpler to just generate exact mappings of this information here.

camkes/templates/label-mapping.thy
@@ -21,7 +21,6 @@ datatype label
 /*- endfor -*/
 (** TPP: condense = False *)
 
-
 (** TPP: condense = True *)
 definition label_of :: "cdl_object_id \<Rightarrow> label option"
   where "label_of \<equiv> empty
@@ -42,6 +41,42 @@ definition id_of :: "string \<Rightarrow> cdl_object_id option"
     /*- endif -*/
   /*- endfor -*/
       None"
+(** TPP: condense = False *)
+
+(** TPP: condense = True *)
+definition ipc_buffer :: "string \<Rightarrow> nat \<Rightarrow> cdl_object_id option"
+  where "ipc_buffer name index \<equiv>
+  /*- set tcbs = {} -*/
+  /*- set to_unfold = set() -*/
+  /*- for i in composition.instances -*/
+    /*- do tcbs.__setitem__('%s_tcb__control' % i.name, (i.name, 0)) -*/
+    /*- for index, inf in enumerate(i.type.provides + i.type.uses + i.type.emits + i.type.consumes + i.type.dataports) -*/
+      /*- do tcbs.__setitem__('%s_tcb_%s' % (i.name, inf.name), (i.name, index + 1)) -*/
+    /*- endfor -*/
+  /*- endfor -*/
+  /*- for o in obj_space.spec.objs -*/
+    /*- if o.name is not none and o.name in tcbs -*/
+      if name = ''/*? tcbs[o.name][0] ?*/'' \<and> index = /*? tcbs[o.name][1] ?*/ then Some /*? o['ipc_buffer_slot'].referent.name ?*/_id else
+      /*- do to_unfold.add('%s_id_def' % o['ipc_buffer_slot'].referent.name) -*/
+    /*- endif -*/
+  /*- endfor -*/
+      None
+  "
+(** TPP: condense = False *)
+
+(** TPP: condense = True *)
+lemma buffers_distinct:
+  "\<And>n i m j. \<exists>f. ipc_buffer n i = Some f \<and> ipc_buffer m j = Some f \<Longrightarrow> n = m \<and> i = j"
+  apply (unfold ipc_buffer_def /*? ' '.join(to_unfold) ?*/)
+  /*- for a in tcbs.values() -*/
+  apply (case_tac "n = ''/*? a[0] ?*/'' \<and> i = /*? a[1] ?*/")
+    /*- for b in tcbs.values() -*/
+   apply (case_tac "m = ''/*? b[0] ?*/'' \<and> j = /*? b[1] ?*/")
+    apply clarsimp
+    /*- endfor -*/
+   apply auto[1]
+  /*- endfor -*/
+  by auto[1]
 (** TPP: condense = False *)
 
 end
